---
author: zc
avatar: null
categories:
- - 刷题记录
commnet: 1
date: 2020-03-12 13:03
html: '<details><summary>查看原题</summary><div id=''from''></div><p><button onclick="document.getElementById(''from'').innerHTML=''<iframe
  src=&quot;http://www.lydsy.com/JudgeOnline/problem.php?id=2956&quot; width=100%
  height=800px style=&quot;border: none;&quot;><iframe>''" class=''mdui-btn mdui-btn-raised
  mdui-ripple''>点击加载</button><a class=''mdui-btn mdui-btn-raised mdui-ripple'' href="http://www.lydsy.com/JudgeOnline/problem.php?id=2956"
  target=''_blank''>点击跳转</a><p></details>'
permalink: BZ 2956 模积和
tags:
- 数论
- 数论分块
thumbnail: null
title: BZ 2956 模积和
top: 0
---
求$\sum_{i=1}^n\sum_{j=1}^m[i≠j](n \bmod i)(m \bmod j),n,m\le 10^9$

数论分块

先不考虑$i!=j$

$$
\sum_{i=1}^n\sum_{j=1}^m(n \bmod i)(m \bmod j)
\\
=\sum_{i=1}^n(n-i\left \lfloor \frac ni\right \rfloor)\sum_{j=1}^m(m-j\left \lfloor \frac mj\right \rfloor)
$$

考虑$i=j$,设$k=\min(n,m)$

$$
\sum_{i=1}^n\sum_{j=1}^m(n \bmod i)(m \bmod j)[i=j]
\\
=\sum_{i=1}^k(n \bmod i)(m \bmod i)
\\
=\sum_{i=1}^k(n-i\left \lfloor \frac ni \right \rfloor)(m-i\left \lfloor \frac mi \right \rfloor)
\\
=\sum_{i=1}^knm-ni\left \lfloor \frac mi \right \rfloor-mi\left \lfloor \frac ni \right \rfloor+i^2 \left \lfloor \frac{nm}{i^2}\right \rfloor
\\
=knm-n\sum_{i=1}^k i\left \lfloor \frac mi \right \rfloor-m\sum_{i=1}^ki\left \lfloor \frac ni \right \rfloor+\sum_{i=1}^ki^2\left \lfloor \frac ni \right \rfloor\left \lfloor \frac mi \right \rfloor
$$

两个相减就是答案

提示: $\sum_{i=1}^n{i^2}=\frac{n(n+1)(2n+1)}6$

> 推导过程: 
> 
> 设$S=\sum_{i=1}^n{i^2}$
> 
> $(n+1)^3-n^3=3n^2+3n+1$
> 
> $n^3-(n-1)^3=3(n-1)^2+3(n-1)+1$
> 
> $\cdots$
> 
> $2^3-1^3=3\times1^2+3\times 1+1$
> 
> 上面$n$个式子相加得到:
> 
> $(n+1)^3-1=3(1^2+2^2+\dots+n^2)+3(1+2+\dots+n)+n$
> 
> $\therefore S=\frac13\left[ (n+1)^3-1- \frac12n(n+1) \right]=\frac{n(n+1)(2n+1)}6$
```cpp
#include<cstdio>
const int P=19940417;
inline int min(int x,int y){return x<y?x:y;}
inline int sum(int l,int r){return 1ll*(l+r)*(r-l+1)/2%P;}
inline int mi(int n){return 1ll*n*(n+1)%P*(2*n+1)%P*3323403%P;}
inline int SUM(int l,int r){return (mi(r)-mi(l-1)+P)%P;}
inline int calc(int k){
    int ans=1ll*k*k%P;
    for(int l=1,r=0;l<=k;l=r+1){
        r=k/(k/l);
        ans=(ans-1ll*sum(l,r)*(k/l)%P+P)%P;
    }
    return ans;
}
int main(){
    int n,m,ans,k;
    scanf("%d%d",&n,&m);
    ans=1ll*calc(n)*calc(m)%P;
    k=min(n,m);
    ans=(ans-1ll*k*n%P*m%P+P)%P;
    for(int l=1,r=0;l<=k;l=r+1){
        r=min(n/(n/l),m/(m/l));
        ans=(ans+1ll*n*sum(l,r)%P*(m/l)%P)%P;
        ans=(ans+1ll*m*sum(l,r)%P*(n/l)%P)%P;
        ans=(ans-1ll*SUM(l,r)*(n/l)%P*(m/l)%P+P)%P;
    }
    printf("%d\n",ans);
}
```
